examples/low-level/MD5.fst
@@ -1,7 +1,8 @@
 (*--build-config
     options:--admit_fsi Set --z3timeout 10;
     variables:LIB=../../lib;
-    other-files:$LIB/ext.fst $LIB/set.fsi $LIB/heap.fst $LIB/st.fst $LIB/list.fst  stack.fst listset.fst st3.fst $LIB/constr.fst word.fst mvector.fsi mvector.fst
+    other-files:$LIB/ext.fst $LIB/set.fsi $LIB/heap.fst $LIB/st.fst $LIB/list.fst  stack.fst listset.fst
+    st3.fst $LIB/constr.fst word.fst mvector.fsi mvector.fst
   --*)
 
 (*Why is MD5 so? Why did its designer(s) think
@@ -10,9 +11,10 @@
   *)
 module MD5
 open StructuredMem
-open MachineWord
 open MVector
-
+open Heap
+open Set
+open MachineWord
 
 (*http://rosettacode.org/wiki/MD5/Implementation#Haskell
  While the version in Haskell and other higher order languages
@@ -65,6 +67,42 @@ let idx n =
   | 2 -> (assert (32<=n/\n<48)); idxH
   | 3 -> (assert (48<=n/\n<64)); idxI
 
+
+
+let rotValues : l:(list (n:nat{n<32}))
+(*{List.length l=16} BUG?*)
+ =
+
+[7; 12; 17; 22;     5; 9; 14; 20;    4; 11; 16; 23;    6; 10; 15; 21]
+
+(*#set-options "--initial_fuel 0 --max_fuel 1000 --initial_ifuel 0 --max_ifuel 1000"*)
+
+
+val lenthRotValue : unit ->
+  Lemma
+      (requires True)
+      (ensures (List.length rotValues = 16))
+[SMTPat rotValues]
+let lenthRotValue u = (admit ())
+
+
+val nthT : #a:Type -> l:(list a) -> n:nat{n<List.length l} -> Tot a
+let rec nthT l n = match l with
+h::tl -> if n=0 then h else (nthT tl (n-1))
+
+val rots: n:nat{n<64} -> Tot (n:nat{n<32})
+let rots n =
+  let row:(n:nat{n<4}) = n/16 in
+  let col:(n:nat{n<4}) = n%4 in
+  let index:(n:nat{n<16}) = row*4+col in
+  nthT rotValues index
+
+(**
+floor(abs(sin(i + 1)) × (2 pow 32))
+*)
+assume val consts: n:nat{n<64} -> Tot word
+
+
 (*add an operation to ref to get a readonly version
   of ref? like const pointers in C++?
   add permission to ref?
@@ -102,6 +140,7 @@ val processChunk :
               /\ refExistsInMem acc m1 /\ ch =!= acc
               (*/\ loopkupRef  ch m0 = loopkupRef ch m1*)
               )
+    (singleton (Ref acc))
 
 let processChunk ch acc =
   let li = salloc #nat 0 in
@@ -112,8 +151,9 @@ let processChunk ch acc =
               /\ refExistsInMem ch m
               /\ refExistsInMem acc m
               /\ refExistsInMem li m /\ loopkupRef li m < 65
-              (*/\ ch =!= acc /\ li =!= acc /\ li =!= ch*)
               )
+    (union (singleton (Ref li)) (singleton (Ref acc)))
+    (*allRefs ; why does this not work?*)
     (fun u ->
       let liv = memread li in
       let vA = readIndex acc iB in
@@ -124,5 +164,7 @@ let processChunk ch acc =
       let g:(n:nat{n<16}) = idx liv liv in
       updIndex acc iD vC;
       updIndex acc iA vD;
-      updIndex acc iB (wmodAdd vA  vC);
+      let mg = readIndex ch g in
+      let vBr = wmodAdd vA  (wmodAdd fF ( wmodAdd(consts liv)  mg)) in
+      updIndex acc iB (wmodAdd vB (leftrotate (rots liv) vBr));
       memwrite li (liv+1))
