examples/low-level/mvector.fst
@@ -8,6 +8,7 @@ module MVector
 open StructuredMem
 open MachineWord
 open Seq
+open Heap
 
 type vector (a:Type) (n:nat) = (index:nat{index<n} -> Tot a)
 
